\documentclass[fleqn]{article}
\usepackage{geometry, mathtools, amssymb, tabularx}
\geometry{portrait, margin=.75in}
\pagestyle{empty}
\begin{document}

\Huge\textbf{Chapter 5}
\vspace{16pt}

\begin{center}
\Large\textbf{5.1 Areas and Distance}

\noindent\hfill\rule{0.3\textwidth}{.4pt}\hfill
\vspace{12pt}

\large
\def\arraystretch{1.3}
{\setlength{\tabcolsep}{16pt}
\begin{tabularx}{.9\textwidth}{|X|}
\hline
	\vspace{1pt}
	The \textbf{area} $A$ of the region $S$ that lies under the graph of the continuous function $f$ is the limit of the sum of the areas of approximating rectangles: \\[10pt]

	$A = \underset{n \to \infty}{\lim} R_n = \underset{n \to \infty}{\lim} [f(x_1) \Delta x + f(x_2) \Delta x + ... + f(x_n) \Delta x]$ \\[10pt]
	$A = \underset{n \to \infty}{\lim} L_n = \underset{n \to \infty}{\lim} [f(x_0) \Delta x + f(x_1) \Delta x + ... + f(x_{n-1}) \Delta x]$ \\[10pt]
	$A = \underset{n \to \infty}{\lim} [f(x_1^*) \Delta x + f(x_2^*) \Delta x + ... + f(x_n^*) \Delta x]$ \\[16pt]
\hline
\end{tabularx}}
\vspace{12pt}

\begin{itemize}
	\item If function is increasing, use left endpoints for underestimation, right endpoints for overestimation. If function is decreasing, use right endpoints for underestimation, left endpoints for overestimation.
	\item Take the height of the $i$th rectangle to be the value of $f$ at any number $x_i^*$ in the $i$th subinterval $[x_{i-1}, x_i]$. The numbers $x_1^*, x_2^*, ... , x_n^*$ are called \textbf{sample points}.
	\item $\Delta x = \dfrac{b-a}{n}$ 
	\item \textbf{Formula for the sum of the squares}: $1^2 + 2^2 +3^2 + ... + n^2 = \dfrac {n(n+1)(2n+1)}{6}$
	\item Use \textbf{sigma notation} to write sums with many terms more compactly. For example:  \[\sum_{i=1}^n f(x_i) \Delta x = f(x_1) \Delta x + f(x_2) \Delta x + ... + f(x_n) \Delta x\]
	\item The formula for the sum of the squares can be rewritten: \[\sum_{i=1}^n i^2 = \dfrac{n(n+1)(2n+1)}{6}\]
	\item The area formulas can be rewritten: 
		\[\text{Right Endpoints: \:\:} A = \underset{n \to \infty}{\lim} \sum_{i=1}^n f(x_i) \Delta x\]
		\[\text{Left Endpoints: \: \hspace{1pt} } A = \underset{n \to \infty}{\lim} \sum_{i=1}^n f(x_{i-1}) \Delta x\]
		\[\text{Midpoints \:\: \hspace{34pt}} A = \underset{n \to \infty}{\lim} \sum_{i=1}^n f(x_i^*) \Delta x\]
%	\item Exact distance $d$ traveled is the limit of the expressions:
%		\[d = \underset{n \to \infty}{lim} \sum_{i=1}^n f(t_{i-1}) \Delta t = \underset{n \to \infty}{\lim} \sum_{i=1}^n f(t) \Delta t\]
\end{itemize}
\end{center}
\pagebreak

\begin{center}
\Large\textbf{5.2 The Definite Integral}

\noindent\hfill\rule{0.3\textwidth}{.4pt}\hfill
\vspace{12pt}

\large
\def\arraystretch{1.3}
{\setlength{\tabcolsep}{16pt}
\begin{tabularx}{.9\textwidth}{|X|}
\hline
	\vspace{1pt}
	If $f$ is a function defined for $a \leq x \leq b$, we divide the interval $[a, b]$ into $n$ subintervals of equal width $\Delta x = (b-a)/n$. We let $x_0(=a), x_1, x_2, ..., x_n(=b)$ be the endpoints of these subintervals and we let $x_1^*, x_2^*, ..., x_n^*$ be any \textbf{sample points} in these subintervals, so $x_i^*$ lies in the $i$th subinterval $[x_{i-1}, x_i]$. Then the \textbf{definite integral of $f$ from $a$ to $b$} is
	$$\int_a^b f(x) dx = \underset{n \to \infty}{\lim} \sum_{i=1}^n f(x_i^*) \Delta x$$
	provided that this limit exists and gives the same value for all possible choices of sample points. If it does exist, we say that $f$ is \textbf{integrable} on $[a,b]$.\\[16pt]
\hline
\end{tabularx}}
\vspace{12pt}

\begin{itemize}
	\item The sum \hspace{3pt} $\sum\limits_{i=1}^n f(x_i^*) \Delta x$ \hspace{3pt} is called a \textbf{Riemann sum}
	\item A definite integral can be interpreted as a \textbf{net area}, that is, a difference of areas:
	$$\int_a^b f(x) dx = A_1 - A_2$$
	where $A_1$ is the area of the region above the $x$-axis and below the graph of $f$, and $A_2$ is the area of the region below the $X$-axis and above the graph of $f$.
\end{itemize}

\def\arraystretch{1.3}
{\setlength{\tabcolsep}{16pt}
\begin{tabularx}{.9\textwidth}{|X|}
\hline
	\vspace{1pt}
	If $f$ is integrable on $[a,b]$, then 
	$$\int_a^b f(x) dx = \underset{n \to \infty}{\lim} \sum_{i=1}^n f(x_i) \Delta x $$
	where \hspace{5pt} $\Delta x = \dfrac{b-a}{n}$ \hspace{5pt} and \hspace{5pt} $x_i = a+i \Delta x$\\[16pt]
\hline
\end{tabularx}}
\vspace{12pt}

\def\arraystretch{1.3}
{\setlength{\tabcolsep}{16pt}
\begin{tabularx}{.9\textwidth}{|X|}
\hline
	\vspace{1pt}
	\textbf{Midpoint Rule}
	$$ \int_a^b f(x) dx \approx \sum_{i=1}^n f(\bar x_i) \Delta x = \Delta x [f(\bar x_1) + ... + f(\bar x_n)] $$ 
	where \hspace{16pt} $\Delta x = \dfrac{b-a}{n}$ \\[12pt]
	and \hspace{30pt} $\bar x_i = \frac{1}{2} (x_{i-1} + x_i)$ \hspace{5pt} = \hspace{5pt} midpoint of \hspace{5pt} $[x_{i-1}, x_i]$ \\[12pt]
\hline
\end{tabularx}}
\vspace{12pt}

\def\arraystretch{1.3}
{\setlength{\tabcolsep}{16pt}
\begin{tabularx}{.9\textwidth}{|X|}
\hline
	\vspace{1pt}
	\textbf{Properties of the Integral}
	\[\int_a^b c \: dx = c(b-a), \text{\hspace{5pt} where $c$ is any constant}\]
	\[\int_a^b [f(x) + g(x)] \: dx = \int_a^b f(x) \: dx + \int_a^b g(x) \: dx\]
	\[\int_a^b c \: f(x) \: dx = c \int_a^b f(x) \: dx, \text{\hspace{5pt} where $c$ is any constant}\]
	\[\int_a^b [f(x) - g(x)] \: dx = \int_a^b f(x) \: dx - \int_a^b g(x) \: dx\]
	\[\int_a^c f(x) \: dx + \int_c^b f(x) \: dx = \int_a^b f(x) \: dx\]\\
	\textbf{Comparison Properties of the Integral} \\[10pt]
	If $f(x) \geq 0$ for $a \leq x \leq b$, then \[\int_a^b f(x) \: dx \geq 0\]
	If $f(x) \geq g(x)$ for $a \leq x \leq b$, then \[\int_a^b f(x) \: dx \geq \int_a^b g(x) \: dx\]
	If $m \leq f(x) \leq M$ for $a \leq x \leq b$, then \[m(b-a) \leq \int_a^b f(x) \: dx \leq M(b-a)\] \\
\hline
\end{tabularx}}
\vspace{12pt}

\def\arraystretch{1.3}
{\setlength{\tabcolsep}{16pt}
\begin{tabularx}{.9\textwidth}{|X|}
\hline
	\vspace{1pt}
	If we reverse $a$ and $b$, then $\Delta x$ changes from $\dfrac{(b-a)}{n}$ to $\dfrac{(a-b)}{n}$. \\ 		Therefore:
	$$ \int_b^a f(x) dx = - \int_a^b f(x) dx $$
	If \hspace{5pt} $a=b$, \hspace{5pt} then \hspace{5pt} $\Delta x = 0$ \hspace{5pt} and so: 
	$$ \int_a^a f(x) dx = 0 $$ \\
\hline
\end{tabularx}}
\vspace{12pt}

\def\arraystretch{.1}
{\setlength{\tabcolsep}{16pt}
\begin{tabularx}{.9\textwidth}{|X X|}
\hline
	\vspace{14pt} \textbf{Formulas for sums of powers} & \vspace{14pt} \textbf{Rules for sigma notation}\\[10pt]
	\[ \sum_{i=1}^n i = \dfrac{n(n+1)}{2} \] & \[ \sum_{i=1}^n c = nc \] \\	
	\[ \sum_{i=1}^n i^2 = \dfrac{n(n+1)(2n+1)}{6} \] & \[ \sum_{i=1}^n ca_i = c \sum_{i=1}^n a_i \] \\
	\[ \sum_{i=1}^n i^3 = \left[ \dfrac{n(n+1)}{2} \right]^2 \] & \[ \sum_{i=1}^n (a_i + b_i) = \sum_{i=1}^n a_i + \sum_{i=1}^n b_i \] \\
	& \[ \sum_{i=1}^n (a_i - b_i) = \sum_{i=1}^n a_i - \sum_{i=1}^n b_i \] \\[5pt]
\hline
\end{tabularx}}
\vspace{12pt}

\vspace{32pt}
\Large\textbf{5.3 The Fundamental Theorem of Calculus}

\noindent\hfill\rule{0.3\textwidth}{.4pt}\hfill
\vspace{12pt}

\large
\def\arraystretch{1.3}
{\setlength{\tabcolsep}{16pt}
\begin{tabularx}{.9\textwidth}{|X|}
\hline
	\textbf{The Fundamental Theorem of Calculus, Part 1} \:\: If $f$ is continuous on $[a,b]$, then the function $g$ defined by 
	$$ g(x) = \int_a^x f(t) dt \text{\hspace{24pt}} a \leq x \leq b$$
	is continuous on $[a,b]$ and differentiable on $(a,b)$ and $g'(x) = f(x)$\\
\hline
\end{tabularx}}
\vspace{12pt}

\def\arraystretch{1.3}
{\setlength{\tabcolsep}{16pt}
\begin{tabularx}{.9\textwidth}{|X|}
\hline
	\textbf{The Fundamental Theorem of Calculus, Part 2} \:\: If $f$ is continuous on $[a,b]$, then 
	$$\int_a^b f(x) dx = F(b) - F(a)$$
	where $F$ is any antiderivative of $f$, that is, a function such that $F' = f$\\
\hline
\end{tabularx}}
\vspace{12pt}

\def\arraystretch{1.3}
{\setlength{\tabcolsep}{16pt}
\begin{tabularx}{.9\textwidth}{|X|}
\hline
	\textbf{The Fundamental Theorem of Calculus} \:\: Suppose $f$ is continuous on $[a,b]$.	
	\[\text{\hspace{-20pt}\textbf{1.} \: If }g(x) = \int_a^x f(t) dt \text{, \hspace{5pt} then }g'(x) = f(x)\]
	\[\text{\textbf{2.} \: }\int_a^b f(x) dx = F(b) - F(a)\text{, where $F$ is any antiderivative of $f$, that is, $F' = f$}\]\\
\hline
\end{tabularx}}
\vspace{12pt}
\pagebreak

\Large\textbf{5.4 Indefinite Integrals and the Net Change Theorem}

\noindent\hfill\rule{0.3\textwidth}{.4pt}\hfill
\vspace{12pt}
\large

\begin{itemize}
	\item The notation $\int f(x) dx$ is traditionally used for an antiderivative of $f$ and is called an \textbf{indefinite integral}. Thus $\int f(x) dx = F(x) \text{ means } F'(x) = f(x)$
	\item Distinguish carefully between definite and indefinite integrals. A definite integral $\int_a^b f(x) dx$ is a \textit{number}, whereas an indefinite integral $\int f(x) dx$ is a \textit{function} (or family of functions).
	\item If $f$ is continuous on $[a,b]$, then $\int_a^b f(x) dx = \int f(x) dx \big|_a^b$
\end{itemize}
\vspace{24pt}

\Large
\def\arraystretch{1.3}
{\setlength{\tabcolsep}{16pt}
\begin{tabularx}{.9\textwidth}{|X X|}
\hline
	\large\textbf{Table of Indefinite Integrals} & \\[5pt]
	$\int cf(x)dx = c \int f(x)dx$ & $\int [f(x) + g(x)]dx =$ \\[10pt]
	$\int k \> dx = kx + C$ & $\int f(x) + \int g(x)dx$ \\[10pt] 
	$\int x^n dx = \dfrac{x^{n+1}}{n+1} + C \hspace{5pt} (n \ne -1)$ & $\int \dfrac{1}{x} dx = ln|x| + C$ \\[10pt]
	$\int e^x dx = e^x + C$ & $\int a^x dx = \dfrac{a^x}{ln \> a} + C$ \\[10pt]
	$\int sinx\>dx = -cosx + C$ & $\int cosx\>dx = sinx +C$ \\[10pt]
	$\int sec^2x\>dx = tanx + C$ & $\int csc^2x\>dx = -cotx + C$ \\[10pt]
	$\int secx\>tanx\>dx = secx +C$ & $\int cscx\>cotx\>dx = -cscx + C$ \\[10pt]
	$\int \dfrac{1}{x^2+1} dx = tan^{-1}x + C$ & $\int \dfrac{1}{\sqrt{1-x^2}} dx = sin^{-1} x + C$ \\[10pt]
	$\int sinhx \> dx = coshx + C$ & $\int coshx \> dx = sinhx + C$\\[10pt]
\hline
\end{tabularx}}
\vspace{24pt}

\large
\def\arraystretch{1.3}
{\setlength{\tabcolsep}{16pt}
\begin{tabularx}{.9\textwidth}{|X|}
\hline
	\vspace{1pt}
	\textbf{Net Change Theorem} \: The integral of a rate of change is the net change:
	$$\int_a^b F'(x)dx = F(b)-F(a)$$\\
\hline
\end{tabularx}}
\vspace{12pt}
\pagebreak

\Large\textbf{5.5 The Substitution Rule}

\noindent\hfill\rule{0.3\textwidth}{.4pt}\hfill
\vspace{12pt}
\large

\def\arraystretch{1.3}
{\setlength{\tabcolsep}{16pt}
\begin{tabularx}{.9\textwidth}{|X|}
\hline
	\vspace{1pt}
	\textbf{The Substitution Rule} \: If $u = g(x)$ is a differentiable function whose range is an interval $I$ and $f$ is continuous on $I$, then
	$$\int f(g(x)) \: g'(x)dx = \int f(u)du$$\\
\hline
\end{tabularx}}
\vspace{12pt}

\def\arraystretch{1.3}
{\setlength{\tabcolsep}{16pt}
\begin{tabularx}{.9\textwidth}{|X|}
\hline
	\vspace{1pt}
	\textbf{The Substitution Rule for Definite Integrals} \: If $g'$ is continuous on $[a,b]$ and $f$ is continuous on the range of $u = g(x)$, then
	$$ \int_a^b f(g(x)) \: g'(x) dx = \int_{g(a)}^{g(b)} f(u) du$$\\
\hline
\end{tabularx}}
\vspace{12pt}

\def\arraystretch{1.3}
{\setlength{\tabcolsep}{16pt}
\begin{tabularx}{.9\textwidth}{|X|}
\hline
	\vspace{1pt}
	\textbf{Integrals of Symmetric Functions} \: Suppose $f$ is continuous on $[-a,a]$.\\[5pt]
	(a) \:\:\: If $f$ is even $[f(-x) = f(x)]$, then $\int_{-a}^a f(x) dx = 2 \int_0^a f(x) dx$\\[5pt]
	(b) \:\:\: If $f$ is odd $[f(-x) = -f(x)]$, then $\int_{-a}^a f(x) dx = 0$\\[14pt]
\hline
\end{tabularx}}
\vspace{12pt}

\end{center}
\end{document}
